module natural where

import Relation.Binary.PropositionalEquality as Eq
open Eq using (_â‰¡_; refl; sym)
open import Data.Bool

data â„• : Set where
  zero : â„•
  suc : â„• â†’ â„•
infixl 6 _+_
_+_ : â„• â†’ â„• â†’ â„•
zero + n = n
suc m + n = suc (m + n)
infixl 7 _*_
_*_ : â„• â†’ â„• â†’ â„•
zero * n = zero
suc m * n = n + (m * n)

pred : â„• â†’ â„•
pred zero = zero
pred (suc n) = n

0+ : âˆ€(x : â„•) â†’ zero + x â‰¡ x
0+ x = refl

+0 : âˆ€(x : â„•) â†’ x + zero â‰¡ x
+0 zero = refl
+0 (suc x) rewrite +0 x = refl

+assoc : âˆ€ (x y z : â„•) â†’ x + (y + z) â‰¡ (x + y) + z
+assoc zero y z = refl
+assoc (suc x) y z rewrite +assoc x y z = refl

+suc : âˆ€ (x y : â„•) â†’ x + suc y â‰¡ suc (x + y)
+suc zero y = refl
+suc (suc x) y rewrite +suc x y = refl

+comm : âˆ€ (x y : â„•) â†’ x + y â‰¡ y + x
+comm zero y rewrite +0 y = refl
+comm (suc x) y rewrite +comm x y | +suc y x = refl

*distrib : âˆ€ (x y z : â„•) â†’ (x + y) * z â‰¡ (x * z) + (y * z)
*distrib zero y z = refl
*distrib (suc x) y z rewrite *distrib x y z | +assoc z (x * z) (y * z) = refl


_<â„•_ : â„• â†’ â„• â†’ Bool
zero <â„• zero = false
zero <â„• suc y = true
suc x <â„• zero = false
suc x <â„• suc y = x <â„• y


_=â„•_ : â„• â†’ â„• â†’ Bool
zero =â„• zero = true
zero =â„• suc y = false
suc x =â„• zero = false
suc x =â„• suc y = x =â„• y


_â‰¤â„•_ : â„• â†’ â„• â†’ Bool
zero â‰¤â„• zero = true
zero â‰¤â„• suc y = true
suc x â‰¤â„• zero = false
suc x â‰¤â„• suc y = x â‰¤â„• y


_â‰¥â„•_ : â„• â†’ â„• â†’ Bool
x â‰¥â„• y = y â‰¤â„• x

_>â„•_ : â„• â†’ â„• â†’ Bool
x >â„• y = y <â„• x

<0 : âˆ€ (x : â„•) â†’ (x <â„• zero) â‰¡ false
<0 zero = refl
<0 (suc x) = refl

ð”¹-contra : false â‰¡ true â†’ âˆ€{l} {P : Set l} â†’ P 
ð”¹-contra ()

<-trans : âˆ€ {x y z : â„•} â†’ (x <â„• y) â‰¡ true â†’ (y <â„• z) â‰¡ true â†’ (x <â„• z) â‰¡ true
<-trans {x} {zero} p1 p2 rewrite <0 x = ð”¹-contra p1
<-trans {zero} {suc y} {zero} p1 () 
<-trans {zero} {suc y} {suc z} p1 p2 = refl
<-trans {suc x} {suc y} {zero} p1 () 
<-trans {suc x} {suc y} {suc z} p1 p2 = <-trans {x} {y} {z} p1 p2

=â„•-to-â‰¡ : âˆ€ {x y : â„•} â†’ x =â„• y â‰¡ true â†’ x â‰¡ y
=â„•-to-â‰¡ {zero} {zero} u = refl
=â„•-to-â‰¡ {suc x} {zero} ()
=â„•-to-â‰¡ {zero} {suc y} ()
=â„•-to-â‰¡ {suc x} {suc y} u rewrite =â„•-to-â‰¡ {x} {y} u = refl

=â„•-refl : âˆ€ (x : â„•) â†’ (x =â„• x) â‰¡ true
=â„•-refl zero = refl
=â„•-refl (suc x) = =â„•-refl x


=â„•-from-â‰¡ : âˆ€ {x y : â„•} â†’ x â‰¡ y â†’ x =â„• y â‰¡ true
=â„•-from-â‰¡ {x} refl = =â„•-refl x

isEven : â„• â†’ Bool
isOdd : â„• â†’ Bool
isEven zero = true
isEven (suc x) = isOdd x
isOdd zero = false
isOdd (suc x) = isEven x

~_ : Bool â†’ Bool
~ true = false
~ false = true

even~odd : âˆ€ (x : â„•) â†’ isEven x â‰¡ ~ isOdd x
odd~even : âˆ€ (x : â„•) â†’ isOdd x â‰¡ ~ isEven x
even~odd zero = refl
even~odd (suc x) = odd~even x
odd~even zero = refl
odd~even (suc x) = even~odd x

+assoc2 : âˆ€ (x y z : â„•) â†’ (x + y) + z â‰¡ x + (y + z)
+assoc2 zero y z = refl
+assoc2 (suc x) y z rewrite +assoc2 x y z = refl

+-swap : âˆ€ (x y z : â„•) â†’ x + (y + z) â‰¡ y + (x + z)
+-swap x y z rewrite sym(+assoc2 y x z) | sym(+assoc2 x y z) | +comm x y = refl

*0 : âˆ€ (x : â„•) â†’ x * zero â‰¡ zero
*0 zero = refl
*0 (suc x) rewrite *0 x = refl

*-suc : âˆ€ (x y : â„•) â†’ x * suc y â‰¡ x + x * y
*-suc zero y = refl
*-suc (suc x) y rewrite *-suc x y | +-swap y x (x * y) = refl

*-comm : (x y : â„•) â†’ x * y â‰¡ y * x
*-comm zero y rewrite *0 y = refl
*-comm (suc x) y rewrite *-suc y x | *-comm x y = refl

+-samex : âˆ€ (x y z : â„•) â†’ y â‰¡ z â†’ x + y â‰¡ x + z
+-samex zero y z p = p 
+-samex (suc x) y z p rewrite +-samex x y z p = refl

*-distri2 : (x y z : â„•) â†’ x * (y + z) â‰¡ x * y + x * z
*-distri2 zero y z = refl
*-distri2 (suc x) y z rewrite *-distri2 x y z | +assoc2 y z (x * y + x * z) | +assoc2 y (x * y) (z + x * z) = +-samex y (z + (x * y + x * z)) (x * y + (z + x * z)) (+-swap z (x * y) (x * z))

-- problem 1.2: associativity of _*_
*-assoc : (x y z : â„•) â†’ (x * y) * z â‰¡ x * (y * z)
*-assoc zero y z = refl
*-assoc (suc x) y z rewrite *-assoc x y z | sym(+assoc2 y z (x * y + x * z)) | *-comm (y + x * y) z | *-distri2 z y (x * y) | *-comm z y | *-comm z (x * y) | sym(*-assoc x y z) = refl

nâ‰®n : (n : â„•) â†’ (n <â„• n) â‰¡ false
nâ‰®n zero = refl 
nâ‰®n (suc n) rewrite nâ‰®n n = refl

-- åå¯¹ç§°æ€§
<-antisym : (x y : â„•) â†’ (x <â„• y) â‰¡ true â†’ (y <â„• x) â‰¡ false
<-antisym zero zero ()
<-antisym (suc x) zero ()
<-antisym zero (suc y) p = refl
<-antisym (suc x) (suc y) p rewrite <-antisym x y p = refl

-- ä¸‰å²æ€§
infix 20 _or_
_or_ : Bool â†’ Bool â†’ Bool
true or _ = true
false or b = b

<-trichotomy : (x y : â„•) â†’ (((x <â„• y) or (x =â„• y)) or (y <â„• x)) â‰¡ true
<-trichotomy zero zero = refl
<-trichotomy (suc x) zero = refl
<-trichotomy zero (suc y) = refl
<-trichotomy (suc x) (suc y) rewrite <-trichotomy x y = refl
